theories/Shallow/Executor.v
@@ -59,60 +59,60 @@ Module Type ShallowExecOn
   (* The main specification monad that we use for execution. It is indexed by
      two program variable contexts Γ1 Γ2 that encode the shape of the program
      variable store before and after execution. *)
-  Definition CHeapSpecM (Γ1 Γ2 : PCtx) (A : Type) : Type :=
+  Definition CStoreSpec (Γ1 Γ2 : PCtx) (A : Type) : Type :=
     (A -> CStore Γ2 -> SCHeap -> Prop) -> CStore Γ1 -> SCHeap -> Prop.
-  Bind Scope mut_scope with CHeapSpecM.
+  Bind Scope mut_scope with CStoreSpec.
 
   Local Open Scope mut_scope.
 
-  Module CHeapSpecM.
+  Module CStoreSpec.
 
     Section Basic.
 
       Definition lift_purem {Γ} {A : Type} :
-        CPureSpec A -> CHeapSpecM Γ Γ A :=
+        CPureSpec A -> CStoreSpec Γ Γ A :=
         fun m POST δ h => m (fun a => POST a δ h).
 
-      Definition pure {Γ A} (a : A) : CHeapSpecM Γ Γ A :=
+      Definition pure {Γ A} (a : A) : CStoreSpec Γ Γ A :=
         fun POST => POST a.
-      Definition bind {Γ1 Γ2 Γ3 A B} (ma : CHeapSpecM Γ1 Γ2 A) (f : A -> CHeapSpecM Γ2 Γ3 B) : CHeapSpecM Γ1 Γ3 B :=
+      Definition bind {Γ1 Γ2 Γ3 A B} (ma : CStoreSpec Γ1 Γ2 A) (f : A -> CStoreSpec Γ2 Γ3 B) : CStoreSpec Γ1 Γ3 B :=
         fun POST => ma (fun a => f a POST).
 
-      Definition error {Γ1 Γ2 A} : CHeapSpecM Γ1 Γ2 A :=
+      Definition error {Γ1 Γ2 A} : CStoreSpec Γ1 Γ2 A :=
         fun POST δ h => FALSE.
-      Definition block {Γ1 Γ2 A} : CHeapSpecM Γ1 Γ2 A :=
+      Definition block {Γ1 Γ2 A} : CStoreSpec Γ1 Γ2 A :=
         fun POST δ h => TRUE.
 
-      Definition demonic_binary {Γ1 Γ2 A} (m1 m2 : CHeapSpecM Γ1 Γ2 A) : CHeapSpecM Γ1 Γ2 A :=
+      Definition demonic_binary {Γ1 Γ2 A} (m1 m2 : CStoreSpec Γ1 Γ2 A) : CStoreSpec Γ1 Γ2 A :=
         fun POST δ h => m1 POST δ h /\ m2 POST δ h.
-      Definition angelic_binary {Γ1 Γ2 A} (m1 m2 : CHeapSpecM Γ1 Γ2 A) : CHeapSpecM Γ1 Γ2 A :=
+      Definition angelic_binary {Γ1 Γ2 A} (m1 m2 : CStoreSpec Γ1 Γ2 A) : CStoreSpec Γ1 Γ2 A :=
         fun POST δ h => m1 POST δ h \/ m2 POST δ h.
 
-      Definition demonic {Γ} (σ : Ty) : CHeapSpecM Γ Γ (Val σ) :=
+      Definition demonic {Γ} (σ : Ty) : CStoreSpec Γ Γ (Val σ) :=
         lift_purem (CPureSpec.demonic σ).
-      Definition angelic {Γ} (σ : Ty) : CHeapSpecM Γ Γ (Val σ) :=
+      Definition angelic {Γ} (σ : Ty) : CStoreSpec Γ Γ (Val σ) :=
         lift_purem (CPureSpec.angelic σ).
 
       Definition angelic_ctx {N : Set} {Γ} :
-        forall Δ : NCtx N Ty, CHeapSpecM Γ Γ (NamedEnv Val Δ) :=
+        forall Δ : NCtx N Ty, CStoreSpec Γ Γ (NamedEnv Val Δ) :=
         fun Δ => lift_purem (CPureSpec.angelic_ctx Δ).
       #[global] Arguments angelic_ctx {N Γ} Δ.
 
-      Definition angelic_list {A Γ} (xs : list A) : CHeapSpecM Γ Γ A :=
+      Definition angelic_list {A Γ} (xs : list A) : CStoreSpec Γ Γ A :=
         lift_purem (CPureSpec.angelic_list xs).
 
-      Definition angelic_finite F `{finite.Finite F} {Γ} : CHeapSpecM Γ Γ F :=
+      Definition angelic_finite F `{finite.Finite F} {Γ} : CStoreSpec Γ Γ F :=
         lift_purem (CPureSpec.angelic_finite F).
       #[global] Arguments angelic_finite F {_ _ Γ}.
 
       Definition demonic_ctx {N : Set} {Γ} :
-        forall Δ : NCtx N Ty, CHeapSpecM Γ Γ (NamedEnv Val Δ) :=
+        forall Δ : NCtx N Ty, CStoreSpec Γ Γ (NamedEnv Val Δ) :=
         fun Δ => lift_purem (CPureSpec.demonic_ctx Δ).
       #[global] Arguments demonic_ctx {N Γ} Δ.
 
     End Basic.
 
-    Module CHeapSpecMNotations.
+    Module CStoreSpecNotations.
 
       Infix "⊗" := demonic_binary (at level 40, left associativity) : mut_scope.
       Infix "⊕" := angelic_binary (at level 50, left associativity) : mut_scope.
@@ -126,21 +126,21 @@ Module Type ShallowExecOn
           (at level 80, ma at level 90, mb at level 200, right associativity) : mut_scope.
       Notation "ma ;; mb" := (bind ma (fun _ => mb)) : mut_scope.
 
-    End CHeapSpecMNotations.
-    Import CHeapSpecMNotations.
+    End CStoreSpecNotations.
+    Import CStoreSpecNotations.
     Local Open Scope mut_scope.
 
     Section AssumeAssert.
 
-      Definition assume_formula {Γ} (fml : Prop) : CHeapSpecM Γ Γ unit :=
+      Definition assume_formula {Γ} (fml : Prop) : CStoreSpec Γ Γ unit :=
         lift_purem (CPureSpec.assume_formula fml).
-      Definition assert_formula {Γ} (fml : Prop) : CHeapSpecM Γ Γ unit :=
+      Definition assert_formula {Γ} (fml : Prop) : CStoreSpec Γ Γ unit :=
         lift_purem (CPureSpec.assert_formula fml).
-      Definition assert_eq_env {Γ} {Δ : Ctx Ty} (δ δ' : Env Val Δ) : CHeapSpecM Γ Γ unit :=
+      Definition assert_eq_env {Γ} {Δ : Ctx Ty} (δ δ' : Env Val Δ) : CStoreSpec Γ Γ unit :=
         lift_purem (CPureSpec.assert_eq_env δ δ').
-      Definition assert_eq_nenv {N Γ} {Δ : NCtx N Ty} (δ δ' : NamedEnv Val Δ) : CHeapSpecM Γ Γ unit :=
+      Definition assert_eq_nenv {N Γ} {Δ : NCtx N Ty} (δ δ' : NamedEnv Val Δ) : CStoreSpec Γ Γ unit :=
         lift_purem (CPureSpec.assert_eq_nenv δ δ').
-      Definition assert_eq_chunk {Γ} (c c' : SCChunk) : CHeapSpecM Γ Γ unit :=
+      Definition assert_eq_chunk {Γ} (c c' : SCChunk) : CStoreSpec Γ Γ unit :=
         lift_purem (CPureSpec.assert_eq_chunk c c').
 
     End AssumeAssert.
@@ -148,12 +148,12 @@ Module Type ShallowExecOn
     Section PatternMatching.
 
       Definition angelic_pattern_match {N : Set} {Γ σ} (pat : @Pattern N σ) (v : Val σ) :
-        CHeapSpecM Γ Γ (MatchResult pat) :=
+        CStoreSpec Γ Γ (MatchResult pat) :=
         lift_purem (CPureSpec.angelic_pattern_match pat v).
       #[global] Arguments angelic_pattern_match {N Γ σ} pat v.
 
       Definition demonic_pattern_match {N : Set} {Γ σ} (pat : @Pattern N σ) (v : Val σ) :
-        CHeapSpecM Γ Γ (MatchResult pat) :=
+        CStoreSpec Γ Γ (MatchResult pat) :=
         lift_purem (CPureSpec.demonic_pattern_match pat v).
       #[global] Arguments demonic_pattern_match {N Γ σ} pat v.
 
@@ -178,25 +178,25 @@ Module Type ShallowExecOn
     Section State.
 
       Definition pushpop {A Γ1 Γ2 x σ} (v : Val σ)
-        (d : CHeapSpecM (Γ1 ▻ x∷σ) (Γ2 ▻ x∷σ) A) : CHeapSpecM Γ1 Γ2 A :=
+        (d : CStoreSpec (Γ1 ▻ x∷σ) (Γ2 ▻ x∷σ) A) : CStoreSpec Γ1 Γ2 A :=
         fun POST δ0 => d (fun a δ1 => POST a (env.tail δ1)) (δ0 ► (x∷σ ↦ v)).
       Definition pushspops {A} {Γ1 Γ2 Δ} (δΔ : CStore Δ)
-        (d : CHeapSpecM (Γ1 ▻▻ Δ) (Γ2 ▻▻ Δ) A) : CHeapSpecM Γ1 Γ2 A :=
+        (d : CStoreSpec (Γ1 ▻▻ Δ) (Γ2 ▻▻ Δ) A) : CStoreSpec Γ1 Γ2 A :=
         fun POST δ0 => d (fun a δ1 => POST a (env.drop Δ δ1)) (δ0 ►► δΔ).
-      Definition get_local {Γ} : CHeapSpecM Γ Γ (CStore Γ) :=
+      Definition get_local {Γ} : CStoreSpec Γ Γ (CStore Γ) :=
         fun POST δ => POST δ δ.
-      Definition put_local {Γ1 Γ2} (δ : CStore Γ2) : CHeapSpecM Γ1 Γ2 unit :=
+      Definition put_local {Γ1 Γ2} (δ : CStore Γ2) : CStoreSpec Γ1 Γ2 unit :=
         fun POST _ => POST tt δ.
-      Definition get_heap {Γ} : CHeapSpecM Γ Γ SCHeap :=
+      Definition get_heap {Γ} : CStoreSpec Γ Γ SCHeap :=
         fun POST δ h => POST h δ h.
-      Definition put_heap {Γ} (h : SCHeap) : CHeapSpecM Γ Γ unit :=
+      Definition put_heap {Γ} (h : SCHeap) : CStoreSpec Γ Γ unit :=
         fun POST δ _ => POST tt δ h.
 
-      Definition eval_exp {Γ σ} (e : Exp Γ σ) : CHeapSpecM Γ Γ (Val σ) :=
+      Definition eval_exp {Γ σ} (e : Exp Γ σ) : CStoreSpec Γ Γ (Val σ) :=
         fun POST δ => POST (eval e δ) δ.
-      Definition eval_exps {Γ} {σs : PCtx} (es : NamedEnv (Exp Γ) σs) : CHeapSpecM Γ Γ (CStore σs) :=
+      Definition eval_exps {Γ} {σs : PCtx} (es : NamedEnv (Exp Γ) σs) : CStoreSpec Γ Γ (CStore σs) :=
         fun POST δ => POST (evals es δ) δ.
-      Definition assign {Γ} x {σ} {xIn : x∷σ ∈ Γ} (v : Val σ) : CHeapSpecM Γ Γ unit :=
+      Definition assign {Γ} x {σ} {xIn : x∷σ ∈ Γ} (v : Val σ) : CStoreSpec Γ Γ unit :=
         fun POST δ => POST tt (δ ⟪ x ↦ v ⟫).
       Global Arguments assign {Γ} x {σ xIn} v.
 
@@ -204,10 +204,10 @@ Module Type ShallowExecOn
 
     Section ProduceConsume.
 
-      Definition produce_chunk {Γ} (c : SCChunk) : CHeapSpecM Γ Γ unit :=
+      Definition produce_chunk {Γ} (c : SCChunk) : CStoreSpec Γ Γ unit :=
         fun POST δ h => POST tt δ (cons c h).
 
-      Definition consume_chunk {Γ} (c : SCChunk) : CHeapSpecM Γ Γ unit :=
+      Definition consume_chunk {Γ} (c : SCChunk) : CStoreSpec Γ Γ unit :=
         h         <- get_heap ;;
         '(c', h') <- angelic_list (heap_extractions h) ;;
         assert_eq_chunk c c' ;;
@@ -216,7 +216,7 @@ Module Type ShallowExecOn
       Global Arguments produce_chunk {Γ} _.
       Global Arguments consume_chunk {Γ} _.
 
-      Fixpoint produce {Γ Σ} (ι : Valuation Σ) (asn : Assertion Σ) : CHeapSpecM Γ Γ unit :=
+      Fixpoint produce {Γ Σ} (ι : Valuation Σ) (asn : Assertion Σ) : CStoreSpec Γ Γ unit :=
         match asn with
         | asn.formula fml => assume_formula (instprop fml ι)
         | asn.chunk c     => produce_chunk (inst c ι)
@@ -235,7 +235,7 @@ Module Type ShallowExecOn
         | asn.debug => pure tt
         end.
 
-      Fixpoint consume {Γ Σ} (ι : Valuation Σ) (asn : Assertion Σ) : CHeapSpecM Γ Γ unit :=
+      Fixpoint consume {Γ Σ} (ι : Valuation Σ) (asn : Assertion Σ) : CStoreSpec Γ Γ unit :=
         match asn with
         | asn.formula fml => assert_formula (instprop fml ι)
         | asn.chunk c     => consume_chunk (inst c ι)
@@ -258,7 +258,7 @@ Module Type ShallowExecOn
 
     Section Exec.
 
-      Definition call_contract {Γ Δ τ} (contract : SepContract Δ τ) (args : CStore Δ) : CHeapSpecM Γ Γ (Val τ) :=
+      Definition call_contract {Γ Δ τ} (contract : SepContract Δ τ) (args : CStore Δ) : CStoreSpec Γ Γ (Val τ) :=
         match contract with
         | MkSepContract _ _ Σe δ req result ens =>
           ι <- angelic_ctx Σe ;;
@@ -269,7 +269,7 @@ Module Type ShallowExecOn
           pure v
         end.
 
-      Definition call_lemma {Γ Δ} (lem : Lemma Δ) (vs : CStore Δ) : CHeapSpecM Γ Γ unit :=
+      Definition call_lemma {Γ Δ} (lem : Lemma Δ) (vs : CStore Δ) : CStoreSpec Γ Γ unit :=
         match lem with
         | MkLemma _ Σe δ req ens =>
           ι <- angelic_ctx Σe ;;
@@ -286,7 +286,7 @@ Module Type ShallowExecOn
          allowed levels before failing execution. Therefore, we write the
          executor in an open-recusion style and [Exec] is the closed type of
          such an executor. *)
-      Definition Exec := forall Γ τ (s : Stm Γ τ), CHeapSpecM Γ Γ (Val τ).
+      Definition Exec := forall Γ τ (s : Stm Γ τ), CStoreSpec Γ Γ (Val τ).
 
       Section ExecAux.
 
@@ -295,7 +295,7 @@ Module Type ShallowExecOn
 
         (* The openly-recursive executor. *)
         Definition exec_aux : Exec :=
-          fix exec_aux {Γ τ} (s : Stm Γ τ) : CHeapSpecM Γ Γ (Val τ) :=
+          fix exec_aux {Γ τ} (s : Stm Γ τ) : CStoreSpec Γ Γ (Val τ) :=
             match s with
             | stm_val _ l => pure l
             | stm_exp e => eval_exp e
@@ -374,7 +374,7 @@ Module Type ShallowExecOn
       Variable inline_fuel : nat.
 
       Definition exec_contract {Δ τ} (c : SepContract Δ τ) (s : Stm Δ τ) :
-       Valuation (sep_contract_logic_variables c) -> CHeapSpecM Δ Δ unit :=
+       Valuation (sep_contract_logic_variables c) -> CStoreSpec Δ Δ unit :=
         match c with
         | MkSepContract _ _ _ _ req result ens =>
           fun ι =>
@@ -392,7 +392,7 @@ Module Type ShallowExecOn
 
     End WithFuel.
 
-  End CHeapSpecM.
+  End CStoreSpec.
 
   Module Replay.
     Import SymProp.
@@ -449,7 +449,7 @@ Module Type ShallowExecOn
   Module Shallow.
 
     Definition ValidContractWithFuel {Δ τ} (fuel : nat) (c : SepContract Δ τ) (body : Stm Δ τ) : Prop :=
-      CHeapSpecM.vcgen fuel c body.
+      CStoreSpec.vcgen fuel c body.
 
     Definition ValidContract {Δ τ} (c : SepContract Δ τ) (body : Stm Δ τ) : Prop :=
       (* Use inline_fuel = 1 by default. *)
