theories/Symbolic/Executor.v
@@ -286,11 +286,11 @@ Module Type SymbolicExecOn
 
   End Configuration.
 
-  Definition SHeapSpecM (Γ1 Γ2 : PCtx) (A : TYPE) : TYPE :=
+  Definition SStoreSpec (Γ1 Γ2 : PCtx) (A : TYPE) : TYPE :=
     □(A -> SStore Γ2 -> SHeap -> 𝕊) -> SStore Γ1 -> SHeap -> 𝕊.
-  Bind Scope mut_scope with SHeapSpecM.
+  Bind Scope mut_scope with SStoreSpec.
 
-  Module SHeapSpecM.
+  Module SStoreSpec.
 
     Local Hint Extern 2 (Persistent (WTerm ?σ)) =>
       refine (@persistent_subst (STerm σ) (@SubstTerm σ)) : typeclass_instances.
@@ -298,67 +298,67 @@ Module Type SymbolicExecOn
     Section Basic.
 
       Definition lift_purem {Γ} {A : TYPE} :
-        ⊢ SPureSpec A -> SHeapSpecM Γ Γ A :=
+        ⊢ SPureSpec A -> SStoreSpec Γ Γ A :=
         fun w0 m POST δ0 h0 =>
           m (fun w1 ω01 a1 => POST w1 ω01 a1 (persist δ0 ω01) (persist h0 ω01)).
 
       Definition pure {Γ} {A : TYPE} :
-        ⊢ A -> SHeapSpecM Γ Γ A := fun _ a k => T k a.
+        ⊢ A -> SStoreSpec Γ Γ A := fun _ a k => T k a.
 
       Definition bind {Γ1 Γ2 Γ3 A B} :
-        ⊢ SHeapSpecM Γ1 Γ2 A -> □(A -> SHeapSpecM Γ2 Γ3 B) -> SHeapSpecM Γ1 Γ3 B :=
+        ⊢ SStoreSpec Γ1 Γ2 A -> □(A -> SStoreSpec Γ2 Γ3 B) -> SStoreSpec Γ1 Γ3 B :=
         fun w0 ma f k => ma (fun w1 ω01 a1 => f w1 ω01 a1 (four k ω01)).
 
       Definition bind_box {Γ1 Γ2 Γ3 A B} :
-        ⊢ □(SHeapSpecM Γ1 Γ2 A) -> □(A -> SHeapSpecM Γ2 Γ3 B) -> □(SHeapSpecM Γ1 Γ3 B) :=
+        ⊢ □(SStoreSpec Γ1 Γ2 A) -> □(A -> SStoreSpec Γ2 Γ3 B) -> □(SStoreSpec Γ1 Γ3 B) :=
         fun w0 m f => bind <$> m <*> four f.
 
       Definition error {Γ1 Γ2 A} :
-        ⊢ (SStore Γ1 -> SHeap -> AMessage) -> SHeapSpecM Γ1 Γ2 A :=
+        ⊢ (SStore Γ1 -> SHeap -> AMessage) -> SStoreSpec Γ1 Γ2 A :=
         fun w msg _ δ h => SymProp.error (msg δ h).
 
       Definition block {Γ1 Γ2 A} :
-        ⊢ SHeapSpecM Γ1 Γ2 A := fun _ POST δ h => block.
+        ⊢ SStoreSpec Γ1 Γ2 A := fun _ POST δ h => block.
 
       Definition angelic_binary {Γ1 Γ2 A} :
-        ⊢ SHeapSpecM Γ1 Γ2 A -> SHeapSpecM Γ1 Γ2 A -> SHeapSpecM Γ1 Γ2 A :=
+        ⊢ SStoreSpec Γ1 Γ2 A -> SStoreSpec Γ1 Γ2 A -> SStoreSpec Γ1 Γ2 A :=
         fun w m1 m2 POST δ1 h1 =>
           angelic_binary (m1 POST δ1 h1) (m2 POST δ1 h1).
       Definition demonic_binary {Γ1 Γ2 A} :
-        ⊢ SHeapSpecM Γ1 Γ2 A -> SHeapSpecM Γ1 Γ2 A -> SHeapSpecM Γ1 Γ2 A :=
+        ⊢ SStoreSpec Γ1 Γ2 A -> SStoreSpec Γ1 Γ2 A -> SStoreSpec Γ1 Γ2 A :=
         fun w m1 m2 POST δ1 h1 =>
           demonic_binary (m1 POST δ1 h1) (m2 POST δ1 h1).
 
       Definition angelic_list {A Γ} :
-        ⊢ (SStore Γ -> SHeap -> AMessage) -> WList A -> SHeapSpecM Γ Γ A :=
+        ⊢ (SStore Γ -> SHeap -> AMessage) -> WList A -> SStoreSpec Γ Γ A :=
         fun w msg xs POST δ h => lift_purem (SPureSpec.angelic_list (msg δ h) xs) POST δ h.
 
       Definition angelic_finite F `{finite.Finite F} {Γ} :
-        ⊢ (SStore Γ -> SHeap -> AMessage) -> SHeapSpecM Γ Γ ⌜F⌝ :=
+        ⊢ (SStore Γ -> SHeap -> AMessage) -> SStoreSpec Γ Γ ⌜F⌝ :=
         fun w msg POST δ h => lift_purem (SPureSpec.angelic_finite F (msg δ h)) POST δ h.
       #[global] Arguments angelic_finite F {_ _ Γ w}.
 
       Definition angelic {Γ} (x : option LVar) :
-        ⊢ ∀ σ, SHeapSpecM Γ Γ (STerm σ) :=
+        ⊢ ∀ σ, SStoreSpec Γ Γ (STerm σ) :=
         fun w σ => lift_purem (SPureSpec.angelic x σ).
       Global Arguments angelic {Γ} x [w] σ : rename.
 
       Definition demonic {Γ} (x : option LVar) :
-        ⊢ ∀ σ, SHeapSpecM Γ Γ (STerm σ) :=
+        ⊢ ∀ σ, SStoreSpec Γ Γ (STerm σ) :=
         fun w σ => lift_purem (SPureSpec.demonic x σ).
       Global Arguments demonic {Γ} x [w] σ : rename.
 
       Definition debug {AT} {Γ1 Γ2} :
-        ⊢ (SStore Γ1 -> SHeap -> AMessage) -> (SHeapSpecM Γ1 Γ2 AT) -> (SHeapSpecM Γ1 Γ2 AT) :=
+        ⊢ (SStore Γ1 -> SHeap -> AMessage) -> (SStoreSpec Γ1 Γ2 AT) -> (SStoreSpec Γ1 Γ2 AT) :=
         fun _ d m POST δ h => SymProp.debug (d δ h) (m POST δ h).
 
       Definition angelic_ctx {N : Set} (n : N -> LVar) {Γ} :
-        ⊢ ∀ Δ : NCtx N Ty, SHeapSpecM Γ Γ (fun w => NamedEnv (Term w) Δ) :=
+        ⊢ ∀ Δ : NCtx N Ty, SStoreSpec Γ Γ (fun w => NamedEnv (Term w) Δ) :=
         fun w Δ => lift_purem (SPureSpec.angelic_ctx n Δ).
       Global Arguments angelic_ctx {N} n {Γ} [w] Δ : rename.
 
       Definition demonic_ctx {N : Set} (n : N -> LVar) {Γ} :
-        ⊢ ∀ Δ : NCtx N Ty, SHeapSpecM Γ Γ (fun w => NamedEnv (Term w) Δ) :=
+        ⊢ ∀ Δ : NCtx N Ty, SStoreSpec Γ Γ (fun w => NamedEnv (Term w) Δ) :=
         fun w Δ => lift_purem (SPureSpec.demonic_ctx n Δ).
       Global Arguments demonic_ctx {N} n {Γ} [w] Δ : rename.
 
@@ -393,15 +393,15 @@ Module Type SymbolicExecOn
 
       (* Add the provided formula to the path condition. *)
       Definition assume_formula {Γ} :
-        ⊢ Formula -> SHeapSpecM Γ Γ Unit :=
+        ⊢ Formula -> SStoreSpec Γ Γ Unit :=
         fun w0 fml => lift_purem (SPureSpec.assume_formula fml).
 
       Definition box_assume_formula {Γ} :
-        ⊢ Formula -> □(SHeapSpecM Γ Γ Unit) :=
+        ⊢ Formula -> □(SStoreSpec Γ Γ Unit) :=
         fun w0 fml => assume_formula <$> persist fml.
 
       Definition assert_formula {Γ} :
-        ⊢ Formula -> SHeapSpecM Γ Γ Unit :=
+        ⊢ Formula -> SStoreSpec Γ Γ Unit :=
         fun w0 fml POST δ0 h0 =>
           lift_purem
             (SPureSpec.assert_formula
@@ -409,11 +409,11 @@ Module Type SymbolicExecOn
             POST δ0 h0.
 
       Definition box_assert_formula {Γ} :
-        ⊢ Formula -> □(SHeapSpecM Γ Γ Unit) :=
+        ⊢ Formula -> □(SStoreSpec Γ Γ Unit) :=
         fun w0 fml => assert_formula <$> persist fml.
 
       Definition assert_pathcondition {Γ} :
-        ⊢ PathCondition -> SHeapSpecM Γ Γ Unit :=
+        ⊢ PathCondition -> SStoreSpec Γ Γ Unit :=
         fun w0 fmls POST δ0 h0 =>
           lift_purem
             (SPureSpec.assert_pathcondition
@@ -428,7 +428,7 @@ Module Type SymbolicExecOn
 
       Definition assert_eq_env {Γ} {Δ : Ctx Ty} :
         let E := fun w : World => Env (Term w) Δ in
-        ⊢ E -> E -> SHeapSpecM Γ Γ Unit :=
+        ⊢ E -> E -> SStoreSpec Γ Γ Unit :=
         fun w0 E1 E2 POST δ0 h0 =>
           lift_purem
             (SPureSpec.assert_eq_env
@@ -444,7 +444,7 @@ Module Type SymbolicExecOn
 
       Definition assert_eq_nenv {N Γ} {Δ : NCtx N Ty} :
         let E := fun w : World => NamedEnv (Term w) Δ in
-        ⊢ E -> E -> SHeapSpecM Γ Γ Unit :=
+        ⊢ E -> E -> SStoreSpec Γ Γ Unit :=
         fun w0 E1 E2 POST δ0 h0 =>
           lift_purem
             (SPureSpec.assert_eq_nenv
@@ -459,12 +459,12 @@ Module Type SymbolicExecOn
             POST δ0 h0.
 
       Definition assert_eq_chunk {Γ} :
-        ⊢ Chunk -> Chunk -> SHeapSpecM Γ Γ Unit :=
+        ⊢ Chunk -> Chunk -> SStoreSpec Γ Γ Unit :=
         fun w0 c1 c2 POST δ0 h0 =>
           lift_purem
             (T (SPureSpec.assert_eq_chunk
                   (amsg.mk
-                     {| msg_function := "SHeapSpecM.assert_eq_chunk";
+                     {| msg_function := "SStoreSpec.assert_eq_chunk";
                         msg_message := "Proof obligation";
                         msg_program_context := Γ;
                         msg_localstore := δ0;
@@ -478,11 +478,11 @@ Module Type SymbolicExecOn
     Section PatternMatching.
 
       Definition angelic_pattern_match {N : Set} (n : N -> LVar) {Γ σ} (pat : @Pattern N σ) :
-        ⊢ STerm σ -> SHeapSpecM Γ Γ (SMatchResult pat) :=
+        ⊢ STerm σ -> SStoreSpec Γ Γ (SMatchResult pat) :=
         fun w0 t Φ δ h =>
           SPureSpec.angelic_pattern_match n pat
             (amsg.mk
-               {| msg_function := "SHeapSpecM.angelic_pattern_match";
+               {| msg_function := "SStoreSpec.angelic_pattern_match";
                  msg_message := "pattern match assertion";
                  msg_program_context := Γ;
                  msg_localstore := δ;
@@ -493,14 +493,14 @@ Module Type SymbolicExecOn
       #[global] Arguments angelic_pattern_match {N} n {Γ σ} pat [w].
 
       Definition demonic_pattern_match {N : Set} (n : N -> LVar) {Γ σ} (pat : @Pattern N σ) :
-        ⊢ STerm σ -> SHeapSpecM Γ Γ (SMatchResult pat) :=
+        ⊢ STerm σ -> SStoreSpec Γ Γ (SMatchResult pat) :=
         fun w0 t Φ δ h =>
           SPureSpec.demonic_pattern_match n pat t
             (fun w1 θ1 mr => Φ w1 θ1 mr δ⟨θ1⟩ h⟨θ1⟩).
       #[global] Arguments demonic_pattern_match {N} n {Γ σ} pat [w].
 
       Definition pattern_match {N : Set} (n : N -> LVar) {Γ σ} (pat : @Pattern N σ) :
-        ⊢ WTerm σ -> SHeapSpecM Γ Γ (SMatchResult pat) :=
+        ⊢ WTerm σ -> SStoreSpec Γ Γ (SMatchResult pat) :=
         fun w t => lift_purem (SPureSpec.new_pattern_match n pat t).
       #[global] Arguments pattern_match {N} n {Γ σ} pat [w].
 
@@ -509,34 +509,34 @@ Module Type SymbolicExecOn
     Section State.
 
       Definition pushpop {AT Γ1 Γ2 x σ} :
-        ⊢ STerm σ -> SHeapSpecM (Γ1 ▻ x∷σ) (Γ2 ▻ x∷σ) AT -> SHeapSpecM Γ1 Γ2 AT :=
+        ⊢ STerm σ -> SStoreSpec (Γ1 ▻ x∷σ) (Γ2 ▻ x∷σ) AT -> SStoreSpec Γ1 Γ2 AT :=
         fun w0 t m POST δ h =>
           m (fun w1 ω01 a1 δ1 => POST w1 ω01 a1 (env.tail δ1)) δ.[x∷σ↦t] h.
 
       Definition pushspops {AT Γ1 Γ2 Δ} :
-        ⊢ SStore Δ -> SHeapSpecM (Γ1 ▻▻ Δ) (Γ2 ▻▻ Δ) AT -> SHeapSpecM Γ1 Γ2 AT :=
+        ⊢ SStore Δ -> SStoreSpec (Γ1 ▻▻ Δ) (Γ2 ▻▻ Δ) AT -> SStoreSpec Γ1 Γ2 AT :=
         fun w0 δΔ m POST δ h =>
           m (fun w1 ω01 a1 δ1 => POST w1 ω01 a1 (env.drop Δ δ1)) (δ ►► δΔ) h.
 
-      Definition get_local {Γ} : ⊢ SHeapSpecM Γ Γ (SStore Γ) :=
+      Definition get_local {Γ} : ⊢ SStoreSpec Γ Γ (SStore Γ) :=
         fun w0 POST δ => T POST δ δ.
-      Definition put_local {Γ1 Γ2} : ⊢ SStore Γ2 -> SHeapSpecM Γ1 Γ2 Unit :=
+      Definition put_local {Γ1 Γ2} : ⊢ SStore Γ2 -> SStoreSpec Γ1 Γ2 Unit :=
         fun w0 δ POST _ => T POST tt δ.
-      Definition get_heap {Γ} : ⊢ SHeapSpecM Γ Γ SHeap :=
+      Definition get_heap {Γ} : ⊢ SStoreSpec Γ Γ SHeap :=
         fun w0 POST δ h => T POST h δ h.
-      Definition put_heap {Γ} : ⊢ SHeap -> SHeapSpecM Γ Γ Unit :=
+      Definition put_heap {Γ} : ⊢ SHeap -> SStoreSpec Γ Γ Unit :=
         fun w0 h POST δ _ => T POST tt δ h.
 
       Definition eval_exp {Γ σ} (e : Exp Γ σ) :
-        ⊢ SHeapSpecM Γ Γ (STerm σ) :=
+        ⊢ SStoreSpec Γ Γ (STerm σ) :=
         fun w POST δ => T POST (peval (seval_exp δ e)) δ.
 
       Definition eval_exps {Γ} {σs : PCtx} (es : NamedEnv (Exp Γ) σs) :
-        ⊢ SHeapSpecM Γ Γ (SStore σs) :=
+        ⊢ SStoreSpec Γ Γ (SStore σs) :=
         fun w POST δ =>
           T POST (env.map (fun (b : PVar∷Ty) (e : Exp Γ (type b)) => peval (seval_exp δ e)) es) δ.
 
-      Definition assign {Γ} x {σ} {xIn : x∷σ ∈ Γ} : ⊢ STerm σ -> SHeapSpecM Γ Γ Unit :=
+      Definition assign {Γ} x {σ} {xIn : x∷σ ∈ Γ} : ⊢ STerm σ -> SStoreSpec Γ Γ Unit :=
         fun w0 t POST δ => T POST tt (δ ⟪ x ↦ t ⟫).
       Global Arguments assign {Γ} x {σ xIn} [w] v.
 
@@ -546,7 +546,7 @@ Module Type SymbolicExecOn
       Import EqNotations.
 
       Definition produce_chunk {Γ} :
-        ⊢ Chunk -> SHeapSpecM Γ Γ Unit :=
+        ⊢ Chunk -> SStoreSpec Γ Γ Unit :=
         fun w0 c k δ h => T k tt δ (cons (peval_chunk c) h).
 
       Fixpoint try_consume_chunk_exact {Σ} (h : SHeap Σ) (c : Chunk Σ) {struct h} : option (SHeap Σ) :=
@@ -628,7 +628,7 @@ Module Type SymbolicExecOn
         end.
 
       Definition consume_chunk {Γ} :
-        ⊢ Chunk -> SHeapSpecM Γ Γ Unit :=
+        ⊢ Chunk -> SStoreSpec Γ Γ Unit :=
         fun w0 c =>
           ⟨ ω1 ⟩ h <- get_heap (w := _) ;;
           match try_consume_chunk_exact h (peval_chunk c⟨ω1⟩) with
@@ -650,7 +650,7 @@ Module Type SymbolicExecOn
           end.
 
       Definition consume_chunk_angelic {Γ} :
-        ⊢ Chunk -> SHeapSpecM Γ Γ Unit :=
+        ⊢ Chunk -> SStoreSpec Γ Γ Unit :=
         fun w0 c =>
           ⟨ ω1 ⟩ h <- get_heap (w := _) ;;
           match try_consume_chunk_exact h (peval_chunk c⟨ω1⟩) with
@@ -677,7 +677,7 @@ Module Type SymbolicExecOn
           end.
 
       Definition produce {Γ} :
-        ⊢ Assertion -> □(SHeapSpecM Γ Γ Unit) :=
+        ⊢ Assertion -> □(SStoreSpec Γ Γ Unit) :=
         fix produce w0 asn :=
           match asn with
           | asn.formula fml => box_assume_formula fml
@@ -710,7 +710,7 @@ Module Type SymbolicExecOn
          end.
 
       Definition consume {Γ} :
-        ⊢ Assertion -> □(SHeapSpecM Γ Γ Unit) :=
+        ⊢ Assertion -> □(SStoreSpec Γ Γ Unit) :=
         fix consume w0 asn :=
           match asn with
           | asn.formula fml => box_assert_formula fml
@@ -749,7 +749,7 @@ Module Type SymbolicExecOn
       Variable cfg : Config.
 
       Definition call_contract {Γ Δ τ} (c : SepContract Δ τ) :
-        ⊢ SStore Δ -> SHeapSpecM Γ Γ (STerm τ) :=
+        ⊢ SStore Δ -> SStoreSpec Γ Γ (STerm τ) :=
         match c with
         | MkSepContract _ _ Σe δe req result ens =>
           fun w0 args =>
@@ -768,7 +768,7 @@ Module Type SymbolicExecOn
        end.
 
       Definition call_lemma {Γ Δ} (lem : Lemma Δ) :
-        ⊢ SStore Δ -> SHeapSpecM Γ Γ Unit :=
+        ⊢ SStore Δ -> SStoreSpec Γ Γ Unit :=
         match lem with
         | MkLemma _ Σe δe req ens =>
           fun w0 args =>
@@ -781,7 +781,7 @@ Module Type SymbolicExecOn
         end.
 
       Definition call_contract_debug {Γ Δ τ} (f : 𝑭 Δ τ) (c : SepContract Δ τ) :
-        ⊢ SStore Δ -> SHeapSpecM Γ Γ (STerm τ) :=
+        ⊢ SStore Δ -> SStoreSpec Γ Γ (STerm τ) :=
         fun w0 δΔ =>
           let o := call_contract c δΔ in
           if config_debug_function cfg f
@@ -808,7 +808,7 @@ Module Type SymbolicExecOn
          number of levels this is allowed before failing execution. Therefore,
          we write the executor in an open-recusion style and [Exec] is the
          closed type of such an executor. *)
-      Definition Exec := forall Γ τ (s : Stm Γ τ), ⊢ SHeapSpecM Γ Γ (STerm τ).
+      Definition Exec := forall Γ τ (s : Stm Γ τ), ⊢ SStoreSpec Γ Γ (STerm τ).
 
       Section ExecAux.
 
@@ -816,7 +816,7 @@ Module Type SymbolicExecOn
         Variable rec : Exec.
 
         (* The openly-recursive executor. *)
-        Definition exec_aux : forall {Γ τ} (s : Stm Γ τ), ⊢ SHeapSpecM Γ Γ (STerm τ) :=
+        Definition exec_aux : forall {Γ τ} (s : Stm Γ τ), ⊢ SStoreSpec Γ Γ (STerm τ) :=
           fix exec_aux {Γ τ} s {w0} :=
             match s with
             | stm_val _ v => pure (term_val τ v)
@@ -883,7 +883,7 @@ Module Type SymbolicExecOn
                 error
                   (fun δ h =>
                      amsg.mk
-                     {| msg_function := "SHeapSpecM.exec";
+                     {| msg_function := "SStoreSpec.exec";
                         msg_message := "stm_bind not supported";
                         msg_program_context := _;
                         msg_localstore := δ;
@@ -913,7 +913,7 @@ Module Type SymbolicExecOn
                    error
                      (fun δ h =>
                         amsg.mk
-                        {| msg_function := "SHeapSpecM.exec";
+                        {| msg_function := "SStoreSpec.exec";
                            msg_message := "out of fuel for inlining";
                            msg_program_context := _;
                            msg_localstore := δ;
@@ -929,7 +929,7 @@ Module Type SymbolicExecOn
       Variable inline_fuel : nat.
 
       Definition exec_contract {Δ τ} (c : SepContract Δ τ) (s : Stm Δ τ) :
-        SHeapSpecM Δ Δ Unit {| wctx := sep_contract_logic_variables c; wco := ctx.nil |} :=
+        SStoreSpec Δ Δ Unit {| wctx := sep_contract_logic_variables c; wco := ctx.nil |} :=
         match c with
         | MkSepContract _ _ _ _ req result ens =>
           ⟨ ω01 ⟩ _   <- produce (w:=@MkWorld _ _) req acc_refl ;;
@@ -947,7 +947,7 @@ Module Type SymbolicExecOn
 
     End Exec.
 
-  End SHeapSpecM.
+  End SStoreSpec.
 
   Module Replay.
 
@@ -1014,7 +1014,7 @@ Module Type SymbolicExecOn
   End Replay.
 
   Module Symbolic.
-    Import SHeapSpecM.
+    Import SStoreSpec.
 
     Definition ValidContractWithFuel {Δ τ} (fuel : nat) (c : SepContract Δ τ) (body : Stm Δ τ) : Prop :=
       VerificationCondition
